code/nist-pcurves/Hacl.Impl.P256.PointAdd.fst
@@ -16,7 +16,7 @@ module S = Spec.P256
 #reset-options "--z3rlimit 50 --fuel 0 --ifuel 0"
 
 inline_for_extraction noextract
-val point_add_1 (t0 t1 t2 t3 t4:felem) (p q:point) : Stack unit
+val point_add_1 {| cp:S.curve_params |} (t0 t1 t2 t3 t4:felem) (p q:point) : Stack unit
   (requires fun h ->
     live h t0 /\ live h t1 /\ live h t2 /\
     live h t3 /\ live h t4 /\ live h p /\ live h q /\
@@ -45,7 +45,7 @@ val point_add_1 (t0 t1 t2 t3 t4:felem) (p q:point) : Stack unit
     fmont_as_nat h1 t2 == t2_s /\ fmont_as_nat h1 t3 == t3_s /\
     fmont_as_nat h1 t4 == t4_s))
 
-let point_add_1 t0 t1 t2 t3 t4 p q =
+let point_add_1 {| cp:S.curve_params |} t0 t1 t2 t3 t4 p q =
   let x1, y1, z1 = getx p, gety p, getz p in
   let x2, y2, z2 = getx q, gety q, getz q in
   fmul t0 x1 x2;
@@ -58,7 +58,7 @@ let point_add_1 t0 t1 t2 t3 t4 p q =
 
 
 inline_for_extraction noextract
-val point_add_2 (t1 t2 t3 t4 t5:felem) (p q:point) : Stack unit
+val point_add_2 {| cp:S.curve_params |} (t1 t2 t3 t4 t5:felem) (p q:point) : Stack unit
   (requires fun h ->
     live h t1 /\ live h t2 /\ live h t3 /\ live h t4 /\ live h t5 /\
     live h p /\ live h q /\
@@ -88,7 +88,7 @@ val point_add_2 (t1 t2 t3 t4 t5:felem) (p q:point) : Stack unit
     fmont_as_nat h1 t3 == t3_s /\ fmont_as_nat h1 t4 == t4_s /\
     fmont_as_nat h1 t5 == t5_s))
 
-let point_add_2 t1 t2 t3 t4 t5 p q =
+let point_add_2 {| cp:S.curve_params |} t1 t2 t3 t4 t5 p q =
   let y1, z1 = gety p, getz p in
   let y2, z2 = gety q, getz q in
   fsub t3 t3 t4;
@@ -100,7 +100,7 @@ let point_add_2 t1 t2 t3 t4 t5 p q =
 
 
 inline_for_extraction noextract
-val point_add_3 (x3 y3 t0 t2:felem) (p q:point) : Stack unit
+val point_add_3 {| cp:S.curve_params |} (x3 y3 t0 t2:felem) (p q:point) : Stack unit
   (requires fun h ->
     live h x3 /\ live h y3 /\ live h t0 /\ live h t2 /\
     live h p /\ live h q /\
@@ -123,7 +123,7 @@ val point_add_3 (x3 y3 t0 t2:felem) (p q:point) : Stack unit
     let y3_s = S.fsub x3_s y3_s in
     fmont_as_nat h1 x3 == x3_s /\ fmont_as_nat h1 y3 == y3_s))
 
-let point_add_3 x3 y3 t0 t2 p q =
+let point_add_3 {| cp:S.curve_params |} x3 y3 t0 t2 p q =
   let x1, z1 = getx p, getz p in
   let x2, z2 = getx q, getz q in
   fadd x3 x1 z1;
@@ -134,7 +134,7 @@ let point_add_3 x3 y3 t0 t2 p q =
 
 
 inline_for_extraction noextract
-val point_add_4 (x3 y3 z3 t1 t2:felem) : Stack unit
+val point_add_4 {| cp:S.curve_params |} (x3 y3 z3 t1 t2:felem) : Stack unit
   (requires fun h ->
     live h x3 /\ live h y3 /\ live h z3 /\ live h t1 /\ live h t2 /\
     LowStar.Monotonic.Buffer.all_disjoint [ loc x3; loc y3; loc z3; loc t1; loc t2 ] /\
@@ -153,7 +153,7 @@ val point_add_4 (x3 y3 z3 t1 t2:felem) : Stack unit
     let y3_s = S.fmul S.b_coeff y3_s in
     fmont_as_nat h1 x3 == x3_s /\ fmont_as_nat h1 y3 == y3_s /\ fmont_as_nat h1 z3 == z3_s))
 
-let point_add_4 x3 y3 z3 t1 t2 =
+let point_add_4 {| cp:S.curve_params |} x3 y3 z3 t1 t2 =
   fmul_by_b_coeff z3 t2;
   fsub x3 y3 z3;
   fdouble z3 x3;
@@ -164,7 +164,7 @@ let point_add_4 x3 y3 z3 t1 t2 =
 
 
 inline_for_extraction noextract
-val point_add_5 (x3 y3 z3 t0 t1 t2:felem) : Stack unit
+val point_add_5 {| cp:S.curve_params |} (x3 y3 z3 t0 t1 t2:felem) : Stack unit
   (requires fun h ->
     live h x3 /\ live h y3 /\ live h z3 /\
     live h t0 /\ live h t1 /\ live h t2 /\
@@ -184,7 +184,7 @@ val point_add_5 (x3 y3 z3 t0 t1 t2:felem) : Stack unit
     let t1_s = S.fadd y3_s y3_s in
     fmont_as_nat h1 t1 == t1_s /\ fmont_as_nat h1 t2 == t2_s /\ fmont_as_nat h1 y3 == y3_s))
 
-let point_add_5 x3 y3 z3 t0 t1 t2 =
+let point_add_5 {| cp:S.curve_params |} x3 y3 z3 t0 t1 t2 =
   fdouble t1 t2;
   fadd t2 t1 t2;
   fsub y3 y3 t2;
@@ -193,7 +193,7 @@ let point_add_5 x3 y3 z3 t0 t1 t2 =
 
 
 inline_for_extraction noextract
-val point_add_6 (x3 y3 z3 t0 t1 t2 t4:felem) : Stack unit
+val point_add_6 {| cp:S.curve_params |} (x3 y3 z3 t0 t1 t2 t4:felem) : Stack unit
   (requires fun h ->
     live h x3 /\ live h y3 /\ live h z3 /\
     live h t0 /\ live h t1 /\ live h t2 /\ live h t4 /\
@@ -219,7 +219,7 @@ val point_add_6 (x3 y3 z3 t0 t1 t2 t4:felem) : Stack unit
     fmont_as_nat h1 t0 == t0_s /\ fmont_as_nat h1 t1 == t1_s /\
     fmont_as_nat h1 t2 == t2_s /\ fmont_as_nat h1 y3 == y3_s))
 
-let point_add_6 x3 y3 z3 t0 t1 t2 t4 =
+let point_add_6 {| cp:S.curve_params |} x3 y3 z3 t0 t1 t2 t4 =
   fadd y3 t1 y3;
   fdouble t1 t0;
   fadd t0 t1 t0;
@@ -229,7 +229,7 @@ let point_add_6 x3 y3 z3 t0 t1 t2 t4 =
 
 
 inline_for_extraction noextract
-val point_add_7 (x3 y3 z3 t0 t1 t2 t3 t4:felem) : Stack unit
+val point_add_7 {| cp:S.curve_params |} (x3 y3 z3 t0 t1 t2 t3 t4:felem) : Stack unit
   (requires fun h ->
     live h x3 /\ live h y3 /\ live h z3 /\
     live h t0 /\ live h t1 /\ live h t2 /\ live h t3 /\ live h t4 /\
@@ -258,7 +258,7 @@ val point_add_7 (x3 y3 z3 t0 t1 t2 t3 t4:felem) : Stack unit
     fmont_as_nat h1 x3 == x3_s /\ fmont_as_nat h1 y3 == y3_s /\
     fmont_as_nat h1 z3 == z3_s /\ fmont_as_nat h1 t1 == t1_s))
 
-let point_add_7 x3 y3 z3 t0 t1 t2 t3 t4 =
+let point_add_7 {| cp:S.curve_params |} x3 y3 z3 t0 t1 t2 t3 t4 =
   fmul y3 x3 z3;
   fadd y3 y3 t2;
   fmul x3 t3 x3;
@@ -269,7 +269,7 @@ let point_add_7 x3 y3 z3 t0 t1 t2 t3 t4 =
 
 
 inline_for_extraction noextract
-val point_add_noalloc: tmp:lbuffer uint64 24ul -> res:point -> p:point -> q:point -> Stack unit
+val point_add_noalloc: {| cp:S.curve_params |} -> tmp:lbuffer uint64 (6ul *. cp.bn_limbs) -> res:point -> p:point -> q:point -> Stack unit
   (requires fun h ->
     live h p /\ live h q /\ live h res /\ live h tmp /\
     eq_or_disjoint p q /\ disjoint q res /\ disjoint p res /\
@@ -280,14 +280,20 @@ val point_add_noalloc: tmp:lbuffer uint64 24ul -> res:point -> p:point -> q:poin
     from_mont_point (as_point_nat h1 res) ==
     S.point_add (from_mont_point (as_point_nat h0 p)) (from_mont_point (as_point_nat h0 q)))
 
-let point_add_noalloc tmp res p q =
+#push-options "--split_queries always"
+let point_add_noalloc {| cp:S.curve_params |} tmp res p q =
   let x3, y3, z3 = getx res, gety res, getz res in
-  let t0 = sub tmp 0ul 4ul in
-  let t1 = sub tmp 4ul 4ul in
-  let t2 = sub tmp 8ul 4ul in
-  let t3 = sub tmp 12ul 4ul in
-  let t4 = sub tmp 16ul 4ul in
-  let t5 = sub tmp 20ul 4ul in
+  let t0 = sub tmp 0ul cp.bn_limbs in
+  let t1 = sub tmp cp.bn_limbs cp.bn_limbs in
+  assert (v (2ul *. cp.bn_limbs) = 2 * v cp.bn_limbs);
+  assert (v (3ul *. cp.bn_limbs) = 3 * v cp.bn_limbs);
+  assert (v (4ul *. cp.bn_limbs) = 4 * v cp.bn_limbs);
+  assert (v (5ul *. cp.bn_limbs) = 5 * v cp.bn_limbs);
+  assert (v (6ul *. cp.bn_limbs) = 6 * v cp.bn_limbs);
+  let t2 = sub tmp (2ul *. cp.bn_limbs) cp.bn_limbs in
+  let t3 = sub tmp (3ul *. cp.bn_limbs) cp.bn_limbs in
+  let t4 = sub tmp (4ul *. cp.bn_limbs) cp.bn_limbs in
+  let t5 = sub tmp (5ul *. cp.bn_limbs) cp.bn_limbs in
   point_add_1 t0 t1 t2 t3 t4 p q;
   point_add_2 t1 t2 t3 t4 t5 p q;
   point_add_3 x3 y3 t0 t2 p q;
@@ -295,14 +301,15 @@ let point_add_noalloc tmp res p q =
   point_add_5 x3 y3 z3 t0 t1 t2;
   point_add_6 x3 y3 z3 t0 t1 t2 t4;
   point_add_7 x3 y3 z3 t0 t1 t2 t3 t4
+#pop-options
 
 
 [@CInline]
-let point_add res p q =
+let point_add {| cp:S.curve_params |} res p q =
   push_frame ();
-  let tmp = create 36ul (u64 0) in
-  let t0 = sub tmp 0ul 24ul in
-  let t1 = sub tmp 24ul 12ul in
+  let tmp = create (9ul *. cp.bn_limbs) (u64 0) in
+  let t0 = sub tmp 0ul (6ul *. cp.bn_limbs) in
+  let t1 = sub tmp (6ul *. cp.bn_limbs) (3ul *. cp.bn_limbs) in
   point_add_noalloc t0 t1 p q;
   copy res t1;
   pop_frame ()
